\documentclass{article}

\usepackage{amsmath,amsfonts,amssymb}
\usepackage[margin=2.6cm]{geometry}
\usepackage{bussproofs}

\input{mathdef.tex}
\input{haskell-lst.tex}

\begin{document}
\title{Normalized Core Language}
\author{suhorng}
\maketitle
\section{Introduction}
\section{Syntax}
\begin{minipage}{\textwidth}
\begin{minipage}[t]{0.33\textwidth}

\begin{code}
v  ::=  $\unit$
    |     $n\in\N$
    |     $b\in\mathbb{B}$
    |     x
\end{code}

\end{minipage}
\begin{minipage}[t]{0.33\textwidth}

\begin{code}
f  ::=  $\Gl$x.e
    |    v v
    |    ref v
    |    !v
    |    v := v
\end{code}

\end{minipage}
\begin{minipage}[t]{0.33\textwidth}

\begin{code}
e  ::=  v
    |    let x = f in e
    |    if v then e$_1$ else e$_2$
\end{code}

\end{minipage}
\end{minipage}
\section{Transforming to NCL}

\section{An Abstract Machine}
\begin{minipage}{\textwidth}
\begin{minipage}[t]{0.50\textwidth}

\subsection{computation}
Let $\Gk' = \langle\mathbf{frame}\; \GG,y,e',\Gk\rangle$.
\begin{itemize}
\item $\langle\GG,\Gs,(\Gl x.e),y,e',\Gk\rangle \longmapsto \langle \Gs,\Gg(\GG,\Gs,\Gl x.e), \Gk'\rangle$
\item $\langle\GG,\Gs,(v_1\;v_2),y,e',\Gk\rangle \longmapsto \langle\GG'',\Gs',e'',\Gk'\rangle$

\begin{itemize}
\item $\langle\mathbf{cl}\; \GG',x',e''\rangle=\Gg(\GG,\Gs,x)$
\item $l\not\in\dom(\Gs)$
\item $\GG''=\GG'[x':= l]$
\item $\Gs'=\Gs[l:= \Gg(\GG,\Gs,v)]$
\end{itemize}

\item $\langle\GG,\Gs,(\mathtt{ref}\; v),y,e',\Gk\rangle \longmapsto \langle\Gs', \langle\mathbf{ref}\; l\rangle,\Gk'\rangle$

\begin{itemize}
  \item $l\not\in\dom(\Gs)$
  \item $\Gs'=\Gs[l:= \Gg(\GG,\Gs,v)]$
\end{itemize}

\item $\langle\GG,\Gs,(\text{\texttt{!}}v),y,e',\Gk\rangle \longmapsto \langle\Gs, \Gs(l),\Gk'\rangle$

\begin{itemize}
\item $\langle\mathbf{ref}\; l\rangle=\Gg(\GG,\Gs,v_1)$ and $l\in\dom(\Gs)$
\end{itemize}

\item $\langle\GG,\Gs,(v_1\; \text{\texttt{:=}}\; v_2),y,e',\Gk\rangle \longmapsto \langle\Gs',\langle\mathbf{unit}\rangle,\Gk'\rangle$

\begin{itemize}
\item $\langle\mathbf{ref}\; l\rangle=\Gg(\GG,\Gs,v_1)$ and $l\in\dom(\Gs)$
\item $\Gs'=\Gs[l:= \Gg(\GG,\Gs,v_2)]$
\end{itemize}
\end{itemize}

\end{minipage}
\begin{minipage}[t]{0.50\textwidth}

\subsection{expressions}
\begin{itemize}
\item $\langle\GG,\Gs,v,\Gk\rangle \longmapsto \langle \Gs,\Gg(\GG,\Gs,v),\Gk \rangle$

\item $\langle\GG,\Gs,(\mathtt{let}\; x=f\; \mathtt{in}\; e),\Gk\rangle \longmapsto \langle\GG,\Gs,f,x, e, \Gk\rangle$

\item $\langle\GG,\Gs,(\mathtt{if}\; v\; \mathtt{then}\; e_1\; \mathtt{else}\; e_2),\Gk\rangle \longmapsto \langle\GG,\Gs, e, \Gk\rangle$

\begin{itemize}
  \item $\displaystyle e = \left\{\begin{array}{rl}
e_1, & \text{if } \Gg(\GG,\Gs,v) = \langle\mathbf{bool}\; \mathit{true}\rangle \\
e_2, & \text{if } \Gg(\GG,\Gs,v) = \langle\mathbf{bool}\; \mathit{false}\rangle
\end{array}\right.$

\end{itemize}
\end{itemize}

\subsection{values}

\begin{itemize}
\item $\langle\Gs,v,\langle\mathbf{frame}\; \GG,x,e,\Gk\rangle\rangle \longmapsto \langle\GG',\Gs',e,\Gk\rangle$
\begin{itemize}
\item $l\not\in\dom(\Gs)$
\item $\GG' = \GG[x:= l]$
\item $\Gs' = \Gs[l:= v]$
\end{itemize}
\end{itemize}

The function $\Gg(\GG,\Gs,v)$ is defined by

\begin{itemize}
  \item $\Gg(\GG,\Gs,\unit) = \langle\mathbf{unit}\rangle$
  \item $\Gg(\GG,\Gs,n) = \langle\mathbf{int}\; n\rangle$
  \item $\Gg(\GG,\Gs,b) = \langle\mathbf{bool}\; b\rangle$
  \item $\Gg(\GG,\Gs,x) = \Gs(\GG(x))$
  \item $\Gg(\GG,\Gs,\Gl x.e) = \langle\mathbf{cl}\; \GG,x,e\rangle$
\end{itemize}

\end{minipage}
\end{minipage}

\end{document}